changes

theories/backtranslation/cast_help/between.v
@@ -1,18 +1,15 @@
-From fae_gtlc_mu.cast_calculus Require Export types consistency.structural.definition.
 From fae_gtlc_mu.stlc_mu Require Export typing lang lib.fix.
-From fae_gtlc_mu.stlc_mu.lib Require Export universe.
-From fae_gtlc_mu.backtranslation Require Export types.
 
 (** Between sums, products, recursive types, arrow types *)
 
 Definition between_TSum (c1 c2 : expr) : expr :=
   Lam (Case (Var 0) (InjL ((rename (+2) c1) (Var 0))) (InjR ((rename (+2) c2) (Var 0)))).
 
-Lemma between_TSum_typed Γ (τ1 τ2 τ1' τ2' : cast_calculus.types.type) (f1 f2 : expr) (d1 : Γ ⊢ₛ f1 : (<<τ1>> → <<τ1'>>)) (d2 : Γ ⊢ₛ f2 : (<<τ2>> → <<τ2'>>)) :
-  Γ ⊢ₛ between_TSum f1 f2 : (<<τ1>> + <<τ2>> → <<τ1'>> + <<τ2'>>)%type.
+Lemma between_TSum_typed Γ (τ1 τ2 τ1' τ2' : type) (f1 f2 : expr) (d1 : Γ ⊢ₛ f1 : (τ1 → τ1')) (d2 : Γ ⊢ₛ f2 : (τ2 → τ2')) :
+  Γ ⊢ₛ between_TSum f1 f2 : (τ1 + τ2 → τ1' + τ2')%type.
 Proof.
   apply Lam_typed.
-  apply Case_typed with (τ1 := <<τ1>>) (τ2 := <<τ2>>).
+  eapply Case_typed.
   by apply Var_typed.
   constructor. eapply App_typed.
   apply up_type_two. apply d1.
@@ -24,8 +21,8 @@ Qed.
 Definition between_TProd (f1 f2 : expr) : expr :=
   Lam (Pair (rename (+1) f1 (Fst (Var 0))) (rename (+1) f2 (Snd (Var 0)))).
 
-Lemma between_TProd_typed Γ (τ1 τ2 τ1' τ2' : cast_calculus.types.type) (f1 f2 : expr) (d1 : Γ ⊢ₛ f1 : (<<τ1>> → <<τ1'>>)) (d2 : Γ ⊢ₛ f2 : (<<τ2>> → <<τ2'>>)) :
-  Γ ⊢ₛ between_TProd f1 f2 : ((<<τ1>> × <<τ2>>) → (<<τ1'>> × <<τ2'>>))%type.
+Lemma between_TProd_typed Γ (τ1 τ2 τ1' τ2' : type) (f1 f2 : expr) (d1 : Γ ⊢ₛ f1 : (τ1 → τ1')) (d2 : Γ ⊢ₛ f2 : (τ2 → τ2')) :
+  Γ ⊢ₛ between_TProd f1 f2 : ((τ1 × τ2) → (τ1' × τ2'))%type.
 Proof.
   apply Lam_typed.
   apply Pair_typed.
@@ -42,47 +39,43 @@ Definition between_TArrow (ca cr : expr) : expr :=
        )
     ).
 
-Lemma between_TArrow_typed Γ (τ1 τ2 τ3 τ4 : cast_calculus.types.type) (ca cr : expr) (da : Γ ⊢ₛ ca : (<<τ3>> → <<τ1>>)) (dr : Γ ⊢ₛ cr : (<<τ2>> → <<τ4>>)) :
-  Γ ⊢ₛ between_TArrow ca cr : ((<<τ1>> → <<τ2>>) → (<<τ3>> → <<τ4>>))%type.
+Lemma between_TArrow_typed Γ (τ1 τ2 τ3 τ4 : type) (ca cr : expr) (da : Γ ⊢ₛ ca : (τ3 → τ1)) (dr : Γ ⊢ₛ cr : (τ2 → τ4)) :
+  Γ ⊢ₛ between_TArrow ca cr : ((τ1 → τ2) → (τ3 → τ4))%type.
 Proof.
   repeat apply Lam_typed.
-  apply App_typed with (τ1 := <<τ2>>).
-  auto. apply up_type_two. apply dr. apply App_typed with (τ1 := <<τ1>>).
+  apply App_typed with (τ1 := τ2).
+  auto. apply up_type_two. apply dr. apply App_typed with (τ1 := τ1).
     by auto; apply Var_typed.
     eapply App_typed. by apply up_type_two.
     by apply Var_typed.
 Qed.
 
 Definition between_TRec (f : expr) : expr :=
-  Lam (* x : μ. <<τi.[...]>> *) (
+  Lam (* x : μ. τi.[...] *) (
       Fix (
-          Lam (* g : μ.<<τi.[...]>> → μ.<<τf.[...]>> *) (
-              Lam (* r : μ.<<τi.[...]>> *) (
-                  Fold (rename (+2) f(*<<τi.[μ.τi/]>>*) (Unfold (Var 0)))
+          Lam (* g : μ.τi.[...] → μ.τf.[...] *) (
+              Lam (* r : μ.τi.[...] *) (
+                  Fold (rename (+1) f(*τi.[μ.τi/]*) (Unfold (Var 0)))
                 )
             )
         ) (Var 0)
     ).
 
-From fae_gtlc_mu.cast_calculus Require Import types. (* make use of subs notation in gtlc *)
-
-Lemma between_TRec_typed Γ (τi τf : cast_calculus.types.type) (Pi : Is_Closed (TRec τi)) (Pf : Is_Closed (TRec τf)) (f : expr)
-      (d : Γ ⊢ₛ f : (<<(τi.[TRec τi/])>> → <<τf.[TRec τf/]>>)) :
-  Γ ⊢ₛ between_TRec f : ((stlc_mu.typing.TRec <<τi>>) → (stlc_mu.typing.TRec <<τf>>))%type.
-From fae_gtlc_mu.stlc_mu Require Export typing.
+Lemma between_TRec_typed Γ (τi τf : type) (Pi : Is_Closed (TRec τi)) (Pf : Is_Closed (TRec τf)) (f : expr)
+      (d : ((TArrow (TRec τi) (TRec τf)):: Γ) ⊢ₛ f : ((τi.[TRec τi/]) → τf.[TRec τf/])) :
+  Γ ⊢ₛ between_TRec f : ((stlc_mu.typing.TRec τi) → (stlc_mu.typing.TRec τf))%type.
 Proof.
   apply Lam_typed.
-  apply App_typed with (τ1 := TRec <<τi>>).
-  apply App_typed with (τ1 := ((TRec << τi >> → TRec << τf >>) → (TRec << τi >> → TRec << τf >>))).
-  apply Fix_typed.
-  admit.
+  apply App_typed with (τ1 := TRec τi).
+  apply App_typed with (τ1 := ((TRec τi → TRec τf) → (TRec τi → TRec τf))).
+  apply Fix_typed; by intro τ; simpl; rewrite -(Pi τ); rewrite -(Pf τ); by simpl.
   apply Lam_typed.
   apply Lam_typed.
   apply Fold_typed.
-  apply App_typed with (τ1 := <<τi>>.[(TRec <<τi>>)/]).
-  apply up_type_two.
-  admit.
+  apply App_typed with (τ1 := τi.[(TRec τi)/]).
+  apply up_type_three.
+  auto.
   apply Unfold_typed.
     by apply Var_typed.
     by apply Var_typed.
-Admitted.
+Qed.
