theories/backtranslation/cast_help/extract.v
@@ -1,6 +1,6 @@
 From fae_gtlc_mu.cast_calculus Require Export types consistency.structural.definition.
-From fae_gtlc_mu.stlc_mu Require Export typing lang lib.fix lib.universe.
-From fae_gtlc_mu.backtranslation Require Export types.
+From fae_gtlc_mu.stlc_mu Require Export typing lang lib.fix.
+From fae_gtlc_mu.backtranslation Require Export types cast_help.universe.
 
 (** Extractions *)
 
