theories/backtranslation/cast_help/factorize.v
@@ -1,7 +1,6 @@
 From fae_gtlc_mu.cast_calculus Require Export types consistency.structural.definition.
 From fae_gtlc_mu.stlc_mu Require Export typing lang lib.fix.
-From fae_gtlc_mu.stlc_mu.lib Require Export universe embed extract.
-From fae_gtlc_mu.backtranslation Require Export types.
+From fae_gtlc_mu.backtranslation.cast_help Require Export universe embed extract.
 
 (** Trivial stuff *)
 
@@ -21,13 +20,13 @@ Definition factorization_up (f : expr) (τG : cast_calculus.types.type) (G : Gro
       embed τG G ((rename (+1) f) (Var 0))
     ).
 
-Lemma factorization_up_typed Γ {f : expr} (τ τG : cast_calculus.types.type) (G : Ground τG) (p1 : (Ground τ -> False)) (p2 : not (τ = ⋆)) (d : Γ ⊢ₛ f : (<<τ>> → <<τG>>)) :
-  Γ ⊢ₛ factorization_up f τG G : (<<τ>> → Universe).
+Lemma factorization_up_typed Γ {f : expr} (τ : type(* backtranslation of something that is not a ground type, nor star *)) (τG : cast_calculus.types.type) (G : Ground τG) (d : Γ ⊢ₛ f : (τ → <<τG>>)) :
+  Γ ⊢ₛ factorization_up f τG G : (τ → Universe).
 Proof.
   apply Lam_typed.
   apply App_typed with (τ1 := << τG >>).
   apply embed_typed.
-  apply App_typed with (τ1 := << τ >>).
+  apply App_typed with (τ1 := τ ).
   apply up_type_one. apply d.
   by apply Var_typed.
 Qed.
@@ -37,8 +36,8 @@ Definition factorization_down (f : expr) (τG : cast_calculus.types.type) (G : G
       (rename (+1) f) (extract τG G (Var 0))
     ).
 
-Lemma factorization_down_typed Γ {f : expr} (τ τG : cast_calculus.types.type) (G : Ground τG) (p1 : notT (Ground τ)) (p2 : not (τ = ⋆)) (d : Γ ⊢ₛ f : (<<τG>> → <<τ>>)) :
-  Γ ⊢ₛ factorization_down f τG G : (Universe → <<τ>>).
+Lemma factorization_down_typed Γ {f : expr} (τ : type(* backtranslation of something that is not a ground type, nor star *)) (τG : cast_calculus.types.type) (G : Ground τG) (d : Γ ⊢ₛ f : (<<τG>> → τ)) :
+  Γ ⊢ₛ factorization_down f τG G : (Universe → τ).
 Proof.
   apply Lam_typed.
   apply App_typed with (τ1 := << τG >>).
